Added other MRDTs

table.py
@@ -1,0 +1,44 @@
+import subprocess
+import time
+from tabulate import tabulate
+
+# Function to execute command and measure time
+def execute_command(command):
+    start_time = time.time()
+    try:
+        subprocess.run(command, shell=True, check=True)
+        #stdout=subprocess.DEVNULL, stderr=subprocess.DEVNULL)
+    except subprocess.CalledProcessError as e:
+        print(f"Error executing the command: {e}")
+        return None
+    end_time = time.time()
+    elapsed_time = end_time - start_time
+    return elapsed_time
+
+# List of commands to execute
+commands = [
+	"fstar.exe mrdts-new/Increment-only_counter/App_new.fst interface/App_new.fsti",
+	"fstar.exe mrdts-new/PN_counter/App_new.fst interface/App_new.fsti",
+	"fstar.exe mrdts-new/Grow-only_set/App_new.fst interface/App_new.fsti interface/Set_extended.fsti",
+	"fstar.exe mrdts-new/Grow-only_map/App_new.fst interface/App_new.fsti interface/Set_extended.fsti interface/Map_extended.fsti",
+	"fstar.exe mrdts-new/Observed-remove_set/App_new.fst interface/App_new.fsti interface/Set_extended.fsti interface/Map_extended.fsti",
+	"fstar.exe mrdts-new/Map/App_new.fst interface/App_new.fsti interface/Set_extended.fsti",
+	"fstar.exe mrdts-new/Enable_wins_flag/App_new.fst interface/App_new.fsti interface/Set_extended.fsti interface/Map_extended.fsti",
+	"fstar.exe mrdts-new/Observed-remove_set_eff_new/App_new_new.fst interface/Set_extended.fsti interface/Map_extended.fsti",
+]
+
+# Execute commands and measure execution time
+results = []
+total_execution_time = 0
+for command in commands:
+    execution_time = execute_command(command)
+    if execution_time is not None:
+        total_execution_time += execution_time
+        results.append([command, f"{execution_time:.4f} seconds"])
+
+# Print individual command execution times in tabular format
+if results:
+    print(tabulate(results, headers=["Command", "Execution Time"]))
+    print(f"\nOverall execution time: {total_execution_time:.4f} seconds")
+else:
+    print("No results to display.")
